wip

proof/scripts/remove_sha256.py
@@ -64,12 +64,6 @@ def remove_functions(input_text: str, template_functions_dict, debug: bool) -> s
         "__core_hash",
         "_core_hash",
         "__core_hash_",
-        # Generic Functions: These are replaced by a single functions that take lists instead of arrays as arguments
-        "__base_w",
-        "__memcpy_u8u8",
-        "_memcpy_u8u8",
-        "_x_memcpy_u8u8",
-        "__memcpy_u8u8_2"
     ]
 
     resolved_functions: list[str] = []
@@ -109,7 +103,7 @@ def remove_functions(input_text: str, template_functions_dict, debug: bool) -> s
         "__prf",
         "__prf_keygen_",
         "__prf_keygen",
-        "_prf_keygen"
+        "_prf_keygen",
     ]
 
     functions_to_remove: list[str] = resolved_functions + regular_functions
@@ -136,110 +130,28 @@ op Hash_ptr : W64.t -> W64.t -> W8.t Array32.t.
 
 op _PRF_ : W8.t Array32.t -> W8.t Array32.t -> W8.t Array32.t -> W8.t Array32.t.
 
-op prf_keygen : W8.t list -> W8.t list -> W8.t list.
+op _PRF_KEYGEN_ : W8.t list -> W8.t list -> W8.t list.
 """
+
     t = text.rfind("module")
     return text[:t] + string_to_add + "\n" + text[t:]
 
-def replace_memcpy(text: str) -> str:
-    return text
 
 def replace_calls(text: str) -> str:
-    """
-    Run 
-        grep -nr "core_hash" | cut -d ' ' -f 4 | uniq | grep -v '^$' 
-    to get this list
-
-    """
-
-    functions: list[str] = [
-        "__core_hash_96",
-        "_core_hash_96",
-        "__core_hash__96",
-        "__core_hash_128",
-        "_core_hash_128",
-        "__core_hash_in_ptr_",
-        "__core_hash_in_ptr",
-        "_core_hash_in_ptr",
-    ]
-
-    for f in functions:
-        pattern = rf"<@ ({f}) \(([^)]+), ([^)]+)\);"
-        replacement = r"<- \1 \2 \3;"
-        text = re.sub(pattern, replacement, text)
-
-    # hash 128
     text = text.replace(
-"""
-  proc __thash_h (out:W8.t Array32.t, in_0:W8.t Array64.t,
-                  pub_seed:W8.t Array32.t, addr:W32.t Array8.t) : W8.t Array32.t *
-                                                                  W32.t Array8.t = {
-    var aux: W8.t Array32.t;
-""",
-"""
-  proc __thash_h (out:W8.t Array32.t, in_0:W8.t Array64.t,
-                  pub_seed:W8.t Array32.t, addr:W32.t Array8.t) : W8.t Array32.t *
-                                                                  W32.t Array8.t = {
-    var aux: W8.t Array32.t;
-    var out_list : W8.t list;
-"""
-    )
-
-    text = text.replace(
-"""
-    out <- _core_hash_128 out buf;
-""",
-"""
-    out_list <- Hash (to_list buf);
-    out <- Array32.of_list witness out_list;
-"""
-    )
-
-    # Hash 96
-    text = text.replace(
-"""
-  proc __thash_f (out:W8.t Array32.t, pub_seed:W8.t Array32.t,
-                  addr:W32.t Array8.t) : W8.t Array32.t * W32.t Array8.t = {
-    var aux: W8.t Array32.t;
-""",
-"""
-  proc __thash_f (out:W8.t Array32.t, pub_seed:W8.t Array32.t,
-                  addr:W32.t Array8.t) : W8.t Array32.t * W32.t Array8.t = {
-    var aux: W8.t Array32.t;
-    var out_list : W8.t list;
-"""
-    )
-
-    text = text.replace(
-"""
-    out <- __core_hash__96 out buf;
-""",
-"""
-
-    out_list <- Hash (to_list buf);    
-    out <- Array32.of_list witness out_list;
-"""
-    )
-
-
-    text = text.replace("__core_hash_in_ptr_", "Hash_ptr")
-    text = text.replace("__core_hash_in_ptr", "Hash_ptr")
-    text = text.replace("_core_hash_in_ptr", "Hash_ptr")
-
-    text = text.replace(
-        "mhash <- Hash_ptr mhash, m_with_prefix_ptr len;", "mhash <- Hash_ptr m_with_prefix_ptr len;"
+        "mhash <@ __core_hash_in_ptr_ (mhash, m_with_prefix_ptr, len);", "mhash <- Hash_ptr m_with_prefix_ptr len;"
     )
 
     text = text.replace(
 """
     aux <@ __prf_ ((Array32.init (fun i_0 => buf.[32 + i_0])), addr_as_bytes,
     pub_seed);
-""",
+ """,
 """
-    aux <- _PRF_ (Array32.init (fun i_0 => buf.[32 + i_0])) addr_as_bytes pub_seed;
+    aux <- _PRF_ (Array32.init (fun i_0 => buf.[32 + i_0])) addr_as_bytes pub_seed; 
 """
-)
-    
+    )
+
     text = text.replace(
 """
     aux <@ __prf_ ((Array32.init (fun i_0 => bitmask.[0 + i_0])),
@@ -251,368 +163,110 @@ def replace_calls(text: str) -> str:
     )
 
     text = text.replace(
-"""
+'''
     aux <@ __prf_ ((Array32.init (fun i_0 => bitmask.[32 + i_0])),
     addr_as_bytes, pub_seed);
-""",
-"""
+''',
+'''
     aux <- _PRF_ (Array32.init (fun i_0 => bitmask.[32 + i_0])) addr_as_bytes pub_seed;
-"""
-    )
-
-    text = text.replace("bitmask <@ __prf_ (bitmask, addr_as_bytes, pub_seed);", "bitmask <- _PRF_ bitmask addr_as_bytes pub_seed;")
-    text = text.replace("buf <@ __prf_ (buf, idx_bytes, sk_prf);", "buf <- _PRF_ buf idx_bytes sk_prf;")
-
-
-    # Replace functions that take arrays as arguments with functions that take lists
-
-    #1) Base W
-
-    text = text.replace (
-"""
-  proc __wots_checksum (csum_base_w:W32.t Array3.t,
-                        msg_base_w:W32.t Array67.t) : W32.t Array3.t = {
-""",
-"""  
-  proc __wots_checksum (csum_base_w:W32.t Array3.t,
-                        msg_base_w:W32.t Array67.t) : W32.t Array3.t = {
-                        
-    var t_list : W32.t list;
-"""
-    )
-    text = text.replace("csum_base_w <@ __base_w_3_2 (csum_base_w, csum_bytes_p);",
-    """
-    t_list <@ BaseWGeneric.__base_w(to_list csum_base_w, to_list csum_bytes_p);
-    csum_base_w <- Array3.of_list witness t_list;
-    """)
-
-    text = text.replace(
-"""
-  proc __chain_lengths (lengths:W32.t Array67.t, msg:W8.t Array32.t) : 
-  W32.t Array67.t = {
-""",
-"""
-  proc __chain_lengths (lengths:W32.t Array67.t, msg:W8.t Array32.t) : 
-  W32.t Array67.t = {
-    var t_list : W32.t list;
-"""
-    )
-
-    text = text.replace("lengths <@ __base_w_67_32 (lengths, msg);",
-    """
-    t_list <@ BaseWGeneric.__base_w(to_list lengths, to_list msg);
-    lengths <- Array67.of_list witness t_list;
-    """)
-
-    # 2) _x_memcpy_u8u8
-    # 2.1 _x_memcpy_u8u8_128_32
-    text = text.replace(
-"""
-  proc __prf_keygen (out:W8.t Array32.t, in_0:W8.t Array64.t,
-                     key:W8.t Array32.t) : W8.t Array32.t = {
-""",
-"""
-  proc __prf_keygen (out:W8.t Array32.t, in_0:W8.t Array64.t,
-                     key:W8.t Array32.t) : W8.t Array32.t = {
-    var buf_list : W8.t list;
-    var in_0_list : W8.t list;
-"""
-    )
-
-    text = text.replace(
-"""
-    (buf,  _0) <@ _x_memcpy_u8u8_128_32 (buf, key);
-""",
-"""
-    (buf_list, _0) <@ Memcpy._x_memcpy_u8u8 (to_list buf, 128, to_list key, 32);
-    buf <- Array128.of_list witness buf_list;
-"""
-    )
-
-    # 2.2 _x_memcpy_u8u8_128_64
-    text = text.replace(
-"""
-    (buf,  _1) <@ _x_memcpy_u8u8_128_64 (buf, offset, in_0);
-""",
-"""
-    (buf_list, _1) <@ Memcpy._x_memcpy_u8u8 (to_list buf, 128, offset, to_list in_0, 64);
-    buf <- Array128.of_list witness buf_list;
-"""
-    )
-
-    # 2.3 _x_memcpy_u8u8_32_32
-    text = text.replace(
-"""
-  proc __gen_chain_inplace (out:W8.t Array32.t, in_0:W8.t Array32.t,
-                            start:W32.t, steps:W32.t,
-                            pub_seed:W8.t Array32.t, addr:W32.t Array8.t) : 
-  W8.t Array32.t * W32.t Array8.t = {
-""",
-"""
-  proc __gen_chain_inplace (out:W8.t Array32.t, in_0:W8.t Array32.t,
-                            start:W32.t, steps:W32.t,
-                            pub_seed:W8.t Array32.t, addr:W32.t Array8.t) : 
-  W8.t Array32.t * W32.t Array8.t = {
-    var out_list : W8.t list;
-"""
-    )
-
-    text = text.replace(
-"""
-    (out,  _0) <@ _x_memcpy_u8u8_32_32 (out, offset, in_0);
-""",
-"""
-    (out_list,  _0) <@ Memcpy._x_memcpy_u8u8 (to_list out, 32, offset, to_list in_0, 32);
-    out <- Array32.of_list witness out_list;
-"""
-    )
-
-    text = text.replace(
-"""
-  proc __expand_seed (outseeds:W8.t Array2144.t, inseed:W8.t Array32.t,
-                      pub_seed:W8.t Array32.t, addr:W32.t Array8.t) : 
-  W8.t Array2144.t * W32.t Array8.t = {
-    var aux_0: int;
-    var aux: W8.t Array32.t;
-""",
-"""
-  proc __expand_seed (outseeds:W8.t Array2144.t, inseed:W8.t Array32.t,
-                      pub_seed:W8.t Array32.t, addr:W32.t Array8.t) : 
-  W8.t Array2144.t * W32.t Array8.t = {
-    var aux_0: int;
-    var aux: W8.t Array32.t;
-    var aux_list: W8.t list;
-"""
-    )
-
-    text = text.replace(
-"""
-    aux <@ _x_memcpy_u8u8_32_32 ((Array32.init (fun i_0 => buf.[0 + i_0])),
-    pub_seed);
-    buf <- Array64.init
-           (fun i_0 => if 0 <= i_0 < 0 + 32 then aux.[i_0-0] else buf.[i_0]);
-""",
-"""
-    aux_list <@ Memcpy._x_memcpy_u8u8 (to_list (Array32.init (fun i_0 => buf.[0 + i_0])),
-    to_list pub_seed);
-    buf <- Array64.init
-           (fun i_0 => if 0 <= i_0 < 0 + 32 then (nth witness aux_list (i_0-0)) else buf.[i_0]);
-"""
-    )
-
-    text = text.replace(
-"""
-  proc __l_tree (leaf:W8.t Array32.t, wots_pk:W8.t Array2144.t,
-                 pub_seed:W8.t Array32.t, addr:W32.t Array8.t) : W8.t Array32.t *
-                                                                 W8.t Array2144.t *
-                                                                 W32.t Array8.t = {
-""",
-"""
-  proc __l_tree (leaf:W8.t Array32.t, wots_pk:W8.t Array2144.t,
-                 pub_seed:W8.t Array32.t, addr:W32.t Array8.t) : W8.t Array32.t *
-                                                                 W8.t Array2144.t *
-                                                                 W32.t Array8.t = {
-    var leaf_list : W8.t list;
-    var buf_0_list : W8.t list;
-    var buf_1_list : W8.t list;
-""" 
-    )
-
-    text = text.replace(
-"""
-    leaf <@ _x_memcpy_u8u8_32_32 (leaf,
-    (Array32.init (fun i_0 => wots_pk.[0 + i_0])));
-""",
-"""
-    leaf_list <@ Memcpy._x_memcpy_u8u8 (to_list leaf,
-    to_list (Array32.init (fun i_0 => wots_pk.[0 + i_0])));
-    leaf <- Array32.of_list witness leaf_list;
-
-"""
-    )
-
-    text = text.replace(
-"""
-  proc __xmssmt_core_seed_keypair (pk:W8.t Array64.t, sk:W8.t Array132.t,
-                                   seed:W8.t Array96.t) : W8.t Array64.t *
-                                                          W8.t Array132.t = {
-""",
-"""
-  proc __xmssmt_core_seed_keypair (pk:W8.t Array64.t, sk:W8.t Array132.t,
-                                   seed:W8.t Array96.t) : W8.t Array64.t *
-                                                          W8.t Array132.t = {
-    var aux_0_list : W8.t list;
-    var aux_1_list : W8.t list;
-"""
-    )
-
-    text = text.replace(
-"""
-    aux_1 <@ _x_memcpy_u8u8_32_32 ((Array32.init (fun i_0 => sk.[(4 + (3 * 32)) + i_0])),
-    (Array32.init (fun i_0 => seed.[(2 * 32) + i_0])));
-""",
-"""
-
-    aux_1_list <@ Memcpy._x_memcpy_u8u8 (to_list (Array32.init (fun i_0 => sk.[(4 + (3 * 32)) + i_0])),
-    to_list (Array32.init (fun i_0 => seed.[(2 * 32) + i_0])));
-    aux_1 <- Array32.of_list witness aux_1_list;
-
-"""
-    )
-
-    text = text.replace(
-"""
-    aux_1 <@ _x_memcpy_u8u8_32_32 ((Array32.init (fun i_0 => pk.[32 + i_0])),
-    (Array32.init (fun i_0 => sk.[(4 + (3 * 32)) + i_0])));
-""",
-"""
-
-    aux_1_list <@ Memcpy._x_memcpy_u8u8(to_list (Array32.init (fun i_0 => pk.[32 + i_0])),
-    to_list (Array32.init (fun i_0 => sk.[(4 + (3 * 32)) + i_0])));
-    aux_1 <- Array32.of_list witness aux_1_list;
+'''
+        )
     
-"""
-    )
-
-    # 2.4 _x_memcpy_u8u8_64_64
     text = text.replace(
-"""
-    aux_0 <@ _x_memcpy_u8u8_64_64 ((Array64.init (fun i_0 => sk.[4 + i_0])),
-    (Array64.init (fun i_0 => seed.[0 + i_0])));
-""",
-"""
-
-    aux_0_list <@ Memcpy._x_memcpy_u8u8(to_list (Array64.init (fun i_0 => sk.[4 + i_0])),
-    to_list (Array64.init (fun i_0 => seed.[0 + i_0])));
-    aux_0 <- Array64.of_list witness aux_0_list;
-
-"""
+'''
+  proc __thash_h (out:W8.t Array32.t, in_0:W8.t Array64.t,
+                  pub_seed:W8.t Array32.t, addr:W32.t Array8.t) : W8.t Array32.t *
+                                                                  W32.t Array8.t = {
+    var aux: W8.t Array32.t;
+''',
+'''
+  proc __thash_h (out:W8.t Array32.t, in_0:W8.t Array64.t,
+                  pub_seed:W8.t Array32.t, addr:W32.t Array8.t) : W8.t Array32.t *
+                                                                  W32.t Array8.t = {
+    var aux: W8.t Array32.t;
+    var out_list : W8.t list;
+'''
     )
-
-    # 2.5 _x_memcpy_u8u8_64_32
+    
     text = text.replace(
-"""
-  proc __compute_root (root:W8.t Array32.t, leaf:W8.t Array32.t,
-                       leaf_idx:W32.t, _auth_path_ptr:W64.t,
-                       pub_seed:W8.t Array32.t, addr:W32.t Array8.t) : 
-  W8.t Array32.t * W32.t Array8.t = {
-""",
-"""
-  proc __compute_root (root:W8.t Array32.t, leaf:W8.t Array32.t,
-                       leaf_idx:W32.t, _auth_path_ptr:W64.t,
-                       pub_seed:W8.t Array32.t, addr:W32.t Array8.t) : 
-  W8.t Array32.t * W32.t Array8.t = {
-    var buffer_list : W8.t list;
-    var aux_list: W8.t list;
-"""
+'''
+    out <@ _core_hash_128 (out, buf);
+''',
+'''
+    out_list <- Hash (to_list buf);
+    out <- Array32.of_list witness out_list;
+'''
     )
 
     text = text.replace(
-"""
-      aux <@ _x_memcpy_u8u8_32_32 ((Array32.init (fun i_0 => buffer.[32 + i_0])),
-      leaf);
-      buffer <- Array64.init
-                (fun i_0 => if 32 <= i_0 < 32 + 32 then aux.[i_0-32]
-                else buffer.[i_0]);
-""",
-"""
-
-      aux_list <@ Memcpy._x_memcpy_u8u8 (to_list (Array32.init (fun i_0 => buffer.[32 + i_0])),
-      to_list leaf);
-
-      buffer <- Array64.init
-                (fun i_0 => if 32 <= i_0 < 32 + 32 then (nth witness aux_list (i_0-32))
-                else buffer.[i_0]);
-
-"""
+'''
+    bitmask <@ __prf_ (bitmask, addr_as_bytes, pub_seed);
+''',
+'''
+    bitmask <-_PRF_ bitmask addr_as_bytes pub_seed;
+'''
     )
 
     text = text.replace(
-"""
-      buffer <@ _x_memcpy_u8u8_64_32 (buffer, leaf);
-""",
-"""
-
-      buffer_list <@ Memcpy._x_memcpy_u8u8 (to_list buffer, to_list leaf);
-      buffer <- Array64.of_list witness buffer_list;
-
-"""
-    )
-
-    # 2.6 __memcpy_u8u8_2144_32
-    text = text.replace(
-"""
-  proc __l_tree (leaf:W8.t Array32.t, wots_pk:W8.t Array2144.t,
-                 pub_seed:W8.t Array32.t, addr:W32.t Array8.t) : W8.t Array32.t *
-                                                                 W8.t Array2144.t *
-                                                                 W32.t Array8.t = {
-""",
-"""
-  proc __l_tree (leaf:W8.t Array32.t, wots_pk:W8.t Array2144.t,
-                 pub_seed:W8.t Array32.t, addr:W32.t Array8.t) : W8.t Array32.t *
-                                                                 W8.t Array2144.t *
-                                                                 W32.t Array8.t = {
-    var wots_pk_list : W8.t list;
-"""
+'''
+  proc __thash_f (out:W8.t Array32.t, pub_seed:W8.t Array32.t,
+                  addr:W32.t Array8.t) : W8.t Array32.t * W32.t Array8.t = {
+    var aux: W8.t Array32.t;
+''',
+'''
+  proc __thash_f (out:W8.t Array32.t, pub_seed:W8.t Array32.t,
+                  addr:W32.t Array8.t) : W8.t Array32.t * W32.t Array8.t = {
+    var aux: W8.t Array32.t;
+    var out_list : W8.t list;
+'''
     )
 
     text = text.replace(
-"""
-        (wots_pk,  _3) <@ __memcpy_u8u8_2144_32 (wots_pk, offset_out, buf0);
-""",
-"""
-        (wots_pk_list, _3) <@ Memcpy._x_memcpy_u8u8(to_list wots_pk, 2144, offset_out, to_list buf0, 32);
-        wots_pk <- Array2144.of_list witness wots_pk_list;
-"""
-    )
+'''
+    out <@ __core_hash__96 (out, buf);
+''',
+'''
 
-    # 5. __memcpy_u8u8_2
-    # NOTE: buf_0_list and buf_1_list are already declared at this point
-    text = text.replace(
-"""
-        (buf0,  _1) <@ __memcpy_u8u8_2_32_2144 (buf0, wots_pk, offset_in,
-        bytes);
-""",
-"""
-        (buf_0_list,  _1) <@ Memcpy.__memcpy_u8u8_2(to_list buf0, to_list wots_pk, offset_in, bytes);
-        buf0 <- Array32.of_list witness buf_0_list;
-"""
+    out_list <- Hash (to_list buf);    
+    out <- Array32.of_list witness out_list;
+'''
     )
 
     text = text.replace(
-"""
-        (buf1,  _2) <@ __memcpy_u8u8_2_64_2144 (buf1, wots_pk, offset_in,
-        bytes);
-""",
-"""
-        (buf_1_list,  _2) <@ Memcpy.__memcpy_u8u8_2(to_list buf1, to_list wots_pk, offset_in, bytes);
-        buf1 <- Array64.of_list witness buf_1_list;
-"""
+'''
+  proc __expand_seed (outseeds:W8.t Array2144.t, inseed:W8.t Array32.t,
+                      pub_seed:W8.t Array32.t, addr:W32.t Array8.t) : 
+  W8.t Array2144.t * W32.t Array8.t = {
+    var aux_0: int;
+    var aux: W8.t Array32.t;
+''',
+'''
+  proc __expand_seed (outseeds:W8.t Array2144.t, inseed:W8.t Array32.t,
+                      pub_seed:W8.t Array32.t, addr:W32.t Array8.t) : 
+  W8.t Array2144.t * W32.t Array8.t = {
+    var aux_0: int;
+    var aux: W8.t Array32.t;
+    var aux_list : W8.t list;
+'''
     )
 
-    # _PRF__KEYGEN
-    text = text.replace(
-"""
-      aux <@ __prf_keygen_ ((Array32.init (fun i_0 => outseeds.[(i * 32) + i_0])),
-      buf, inseed);
-""",
-"""
-      aux_list <- prf_keygen (to_list buf) (to_list inseed);
-      aux <- Array32.of_list witness aux_list;
-"""
-    )
+    text = text.replace('ith_seed <@ __prf_keygen_ (ith_seed, buf, inseed);', 
+'''
+    aux_list <- _PRF_KEYGEN_ (to_list buf) (to_list inseed);
+    ith_seed <- Array32.of_list witness aux_list;
+''')
+
+    text = text.replace('buf <@ __prf_ (buf, idx_bytes, sk_prf);', 'buf <- _PRF_ buf idx_bytes sk_prf;')
 
     return text
 
-########################################################################################################################
-
 
 def preprocess_ec(ec_in: str, template_functions_dict, debug: bool) -> str:
-    ec_out = ec_in.replace("module M", "module Mp")
+    ec_out = ec_in.replace("module M(SC:Syscall_t)", "module Mp(SC:SCall_t)")
 
-        # Remove module related to randombytes
+    # Rename module related to randombytes
     ec_out = ec_out.replace(
-"""
+        """
 module type Syscall_t = {
   proc randombytes_96(_:W8.t Array96.t) : W8.t Array96.t
 }.
@@ -625,15 +279,27 @@ module Syscall : Syscall_t = {
   }
 }.
 """,
-        ""
+        """
+module type SCall_t = {
+  proc randombytes_96(_:W8.t Array96.t) : W8.t Array96.t
+}.
+
+module SCall : SCall_t = {
+  proc randombytes_96(a:W8.t Array96.t) : W8.t Array96.t = {
+    a <$ dmap WArray96.darray
+         (fun a => Array96.init (fun i => WArray96.get8 a i));
+    return a;
+  }
+}.
+""",
     )
+
+    ec_out = ec_out.replace("(* Erased call to spill *)", "")
+    ec_out = ec_out.replace("(* Erased call to unspill *)", "")
 
     ec_out = remove_functions(ec_out, template_functions_dict, debug)
     ec_out = add_operators(ec_out)
     ec_out = replace_calls(ec_out)
-
-    ec_out = ec_out.replace("(* Erased call to spill *)", "")
-    ec_out = ec_out.replace("(* Erased call to unspill *)", "")
 
     ec_out = re.sub(r"\n\s*\n+", "\n\n", ec_out)  # Remove whitespace
     ec_out = re.sub(r"else\s*{\s*}", "", ec_out)  # Remove empty else statements
