proof/correctness/Correctness_Mem.ec
@@ -4,8 +4,8 @@ require import AllCore List RealExp IntDiv.
 
 from Jasmin require import JModel.
 
-require import Array4 Array32 Array128.
-require import XMSS_IMPL XMSS_IMPL_PP.
+require import Array4 Array32 Array128 Array2144.
+require import XMSS_IMPL (* XMSS_IMPL_PP *).
 
 require import Utils. (* valid_ptr predicate *)
 
@@ -42,7 +42,7 @@ while (
 qed.
 
 lemma memset_zero_post (x : W8.t Array4.t) :
-    hoare [Mp(Syscall).__memset_zero_u8 : true ==> forall (k : int), 0 <= k < 4 => (res.[k] = W8.zero)].
+    hoare [M(Syscall).__memset_zero_u8 : true ==> forall (k : int), 0 <= k < 4 => (res.[k] = W8.zero)].
 proof.
 proc.
 while (
@@ -58,16 +58,17 @@ lemma load_store  (mem : global_mem_t) (ptr : W64.t) (v : W8.t) :
       by rewrite /storeW8 /loadW8 get_setE ifT.
 
 lemma memset_ptr_post (ptr : W64.t, len : W64.t, v : W8.t) :
-    hoare [Mp(Syscall).__memset_u8_ptr : 
+    hoare [M(Syscall).__memset_u8_ptr : 
       0 <= to_uint len /\
       0 <= to_uint ptr /\ to_uint (ptr + len) < W64.modulus /\ 
       arg=(ptr, len, v) ==>
         forall (k:int), 0 <= k < to_uint len => (loadW8 Glob.mem (W64.to_uint (ptr  + (W64.of_int k)))) = v].
 proof.
-proc.
-auto.
+proc ; auto.
 while (
-  #pre /\
+  0 <= to_uint len /\
+  0 <= to_uint ptr /\ 
+  to_uint (ptr + len) < W64.modulus /\ 
   inlen = len /\ value = v /\ _ptr = ptr /\
   0 <= to_uint i <= to_uint inlen /\
   (forall (k : int), 0 <= k < to_uint i => loadW8 Glob.mem ((W64.to_uint _ptr) + k) = v )
@@ -84,26 +85,25 @@ qed.
 (******************************************************************************)
 (******************               MEMCPY                          *************)
 (******************************************************************************)
+
 lemma memcpy_ptr_correct (ptr : W64.t):
-    hoare [Mp(Syscall)._x_memcpy_u8u8p : 
+    hoare [M(Syscall)._x_memcpy_u8u8p : 
       arg.`2 = ptr /\  
       0 <= (to_uint ptr) + 32 <= W64.modulus /\
       0 <= to_uint ptr ==>
         res = Array32.init (fun (i : int) => loadW8 Glob.mem (to_uint ptr + i))].
 proof.
 proc.
-inline *.
-wp ; sp.
+inline * ; wp ; sp.
 while (
   0 <= i <= 32 /\
   0 <= to_uint in_ptr{hr} + 32 <= W64.modulus /\
   forall (k : int), 0 <= k < i => (out1.[k] = loadW8 Glob.mem ((to_uint ptr) + k))
 ) ; auto => />; last first.
-- move => &hr *. split ; first by smt(@JMemory). move => *. apply tP ; smt(@JMemory @Array32).
-- move => &hr *. split ; first by smt(). move => k *. rewrite get_setE 1:/#. case (k = i{hr}); last by smt(@JMemory).
+- move => &hr *. split ; 1:smt(@JMemory). move => *. rewrite tP ; smt(@JMemory @Array32).
+- move => &hr *. split ; 1:smt(). move => k *. rewrite get_setE 1:/#. case (k = i{hr}); last by smt(@JMemory).
   move => E0 ; congr. rewrite E0 to_uintD of_uintK //=. admit. (* overflow *)
 qed.
-
 
 lemma  memcpy_post (x : W8.t Array32.t) :
     hoare [M(Syscall).__memcpy_u8u8_32_32 : arg.`2 = x ==> res = x].
@@ -113,8 +113,8 @@ while (
   0 <= to_uint i <= 32 /\
   (forall (k : int), 0 <= k < to_uint i => (out.[k] = in_0.[k]))
 ); last first.
-- auto => /> *. split ; first by smt(). progress. rewrite tP. move => *. smt.
-- auto => /> &hr *. do split; 1,2: by smt(@W64). move => k *. rewrite get_setE. smt(@W64). case (k = to_uint i{hr}).
+- auto => /> *. split ; 1:smt(). progress. rewrite tP. move => *. smt.
+- auto => /> &hr *. do split; 1,2:smt(@W64). move => k *. rewrite get_setE. smt(@W64). case (k = to_uint i{hr}).
     + move => E0 ; by rewrite E0.
     + move => E0. smt.
 qed.
@@ -123,7 +123,63 @@ lemma _x_memcpy_u8u8_post (x : W8.t Array32.t) :
     hoare [M(Syscall)._x_memcpy_u8u8_32_32 : arg.`2 = x ==> res = x].
 proof.
 proc ; inline M(Syscall)._memcpy_u8u8_32_32.
+wp ; sp ; ecall (memcpy_post in_00) ; skip => />.
+qed.
+
+
+(******************************************************************************)
+(******************               MEMCMP                          *************)
+(******************************************************************************)
+
+lemma memcmp_true (x y : W8.t Array32.t) :
+    x = y => 
+        hoare[M(Syscall).__memcmp : arg = (x, y) ==> res = W64.zero].
+proof.
+move => xy_eq.
+proc ; auto => /> *.
+while(0 <= to_uint i <= 32 /\  a = b /\  acc = W8.zero) ; auto => /> *; smt(@W64).
+qed.
+
+lemma memcmp_false (x y : W8.t Array32.t) :
+    x <> y => 
+        hoare[M(Syscall).__memcmp : arg = (x, y) ==> res = W64.of_int (-1)].
+proof.
+move => xy_neq.
+proc.
+seq 6: (!zf /\ r = W64.of_int (-1)) ; last by auto => />.
 wp ; sp.
-ecall (memcpy_post in_00).
-skip => /> *.
+while (
+  0 <= to_uint i <= 32 /\ a <> b
+(*  (acc = W8.zero => (forall (j : int), 0 <= j < to_uint i => a.[j] = b.[j])) *)
+) ; auto => /> *.
+- smt(@W64).
+- admit.
+qed.
+
+(* INLEN = 32 /\ OUTLEN = 2144 *)
+(* pre: copying all elements of in does not write out of bounds in out *)
+(* 0 <= offset + 32 <= 2144 *)
+(* 0 <= offset <= 2112 *)
+(* same as memcpy(out + offset, in, sizeof(in)); *)
+lemma memcpy_offset_1 (_out_ : W8.t Array2144.t, _offset_ : W64.t, _in_ : W8.t Array32.t) :
+    hoare [M(Syscall).__memcpy_u8u8_offset : 
+      arg.`2=_offset_ /\ arg.`3=_in_ /\  0 <= to_uint _offset_ <= 2122 ==>
+        (forall (k : int), 0 <= k < 32 => (res.[to_uint _offset_ + k] = _in_.[k]))].
+proof.
+proc.
+sp.
+while (
+  0 <= to_uint offset <= 2144 /\ (* offset + inlen <= outlen *)
+  0 <= to_uint i <= 32 /\
+  forall (k : int), 0 <= k < 32 => (out.[to_uint _offset_ + k] = in_0.[k])
+) ; last first.
+- skip => /> &hr * ; do split.
+    + smt(@W64 pow2_64).
+    + move => ???. admit. (* smt(@Array32 @Array2144). *) 
+- auto => /> &hr * ; do split.
+    + smt(@W64).
+    + move => ?.  admit.
+    + smt(@W64).
+    + smt(@W64).
+    + move => ???. rewrite get_setE. split ; 1:smt(). move => ?. admit. admit.
 qed.
